WIP:sp_stree lemmas prooved

x86/Asm.v
@@ -342,6 +342,178 @@ Fixpoint set_res (res: builtin_res preg) (v: val) (rs: regset) : regset :=
   | BR_splitlong hi lo => set_res lo (Val.loword v) (set_res hi (Val.hiword v) rs)
   end.
 
+Definition aligned_fsz (sz:Z) := align (Z.max 0 sz) 8.
+
+Definition check_topframe (sz:Z)(astack:stackadt) : bool :=
+  match astack with
+    |nil => false
+    |top::tl => match top with
+                |fr::nil => if (zeq (aligned_fsz sz) (frame_size_a fr)) then true else false
+                |_ => false
+              end
+  end.
+
+Fixpoint sp_of_stack' (s:stree) : list fid * path :=
+  match s with
+   |Node fid bl l None => (fid::nil,nil)
+   |Node fid bl l (Some s') =>
+    let (lf',path') := sp_of_stack' s' in let idx := length l in
+    (lf'++(fid::nil),idx::path')
+  end.
+
+Lemma sp_of_stack'_nonempty : forall s lf p, sp_of_stack' s= (lf,p) -> lf <> nil.
+Proof.
+  intros. destruct s. destruct o; simpl in H. destr_in H; inv H.
+  intro. destruct l1 in H; inv H. inv H. congruence .
+Qed.
+
+(* we have to ignore the root node*)
+Definition sp_of_stack (s:stree) : list fid * path :=
+  let (lf,path) := (sp_of_stack' s) in (removelast lf,path).
+
+Definition parent_sp_stree (st:stree) : val :=
+  let (lf,path) := sp_of_stack st in
+  match (lf,path) with
+    |(f1::((Some id)::tl), _::(_::_)) =>
+     Vptr (Stack (Some id) (removelast path) 1%positive) Ptrofs.zero
+    |_ => Vnullptr
+  end.
+
+Definition top_sp_stree (st:stree) : val :=
+  let (lf,path) := sp_of_stack st in
+  match (lf,path) with
+    | (((Some id)::tl), (_::_)) =>
+     Vptr (Stack (Some id) path 1%positive) Ptrofs.zero
+    |_ => Vnullptr
+  end.
+
+Lemma sp_of_stack_pspnull : forall st fid idx,
+    sp_of_stack st = (fid::nil,idx::nil) -> parent_sp_stree st = Vnullptr.
+Proof.
+  intros. unfold parent_sp_stree. rewrite H. auto.
+Qed.
+
+Lemma append_nil_right : forall A (l:list A),
+    l++nil = l.
+Proof.
+  induction l. auto. simpl. congruence.
+Qed.
+
+Lemma sp_of_stack_pspsome : forall st f1 lf path idx2 idx1 id,
+    sp_of_stack st = (f1::(Some id)::lf, (path++(idx2::nil))++(idx1::nil)) ->
+    parent_sp_stree st = Vptr (Stack (Some id) (path++(idx2::nil)) 1%positive) Ptrofs.zero.
+Proof.
+  intros. unfold parent_sp_stree. rewrite H. simpl.
+  destruct path. auto. destruct path. auto. rewrite removelast_app. simpl.
+  rewrite append_nil_right. auto. congruence.
+Qed.
+
+Lemma sp_of_stack_return' : forall st st' p' fid lf path idx root,
+    return_stree st = Some (st',p') ->
+    sp_of_stack' st = (fid::lf++(root::nil),path++(idx::nil)) ->
+    sp_of_stack' st' = (lf++(root::nil),path).
+Proof.
+  induction st. intros. destruct st. destruct o.
+  - destruct st'. destruct s. destruct o0.
+    + remember (Node f1 l3 l4 (Some s)) as st1.
+      simpl in H0. destr_in H0. destr_in H0. subst p.
+      simpl in H1. destr_in H1. inv H1.
+      destruct l5. inv H3. destruct lf; inv H5.
+      assert (l5<>nil).
+      {destruct l5.
+      simpl in Heqp. destr_in Heqp. destruct s. destruct o0; simpl in Heqp1.
+      -- destr_in Heqp1. inv Heqp1. destruct l8; inv Heqp. simpl in H5. destruct l8; inv H5.
+      -- inv Heqp1. inv Heqp.
+      -- congruence.
+      }
+      apply exists_last in H1. destruct H1 as (l' & root' & H1). subst.
+      assert (p<> nil).
+      {
+        simpl in Heqp. destr_in Heqp.
+      }
+      apply exists_last in H1. destruct H1 as (path0 & idx' & H1). subst.
+      exploit H; eauto. simpl. auto. intro.
+      inv H0. simpl. rewrite H1.
+      assert (removelast ((Datatypes.length l2 :: path0) ++ idx'::nil) = removelast (path++idx::nil)).
+      setoid_rewrite H4. auto.
+      rewrite removelast_app in H0. simpl in H0. rewrite removelast_app in H0. simpl in H0.
+      repeat rewrite append_nil_right in H0. subst.
+      assert (tl ((f2::l'++root'::nil)++f0::nil) = tl (fid::lf++root::nil)).
+      setoid_rewrite H3. auto. simpl in H0. rewrite H0. auto. congruence. congruence.
+      rewrite Heqst1 in Heqo0. inv Heqo0. repeat destr_in H3.
+    + simpl in H1. simpl in H0. inv H0.
+      simpl in *.  inv H1. destruct path; inv H4. auto.
+      destruct path; inv H2.
+  - inv H1. destruct lf; inv H4.
+Qed.
+
+Lemma sp_of_stack_return : forall m1 m2 fid lf path idx,
+    Mem.return_frame m1 = Some m2 ->
+    sp_of_stack (Mem.stack (Mem.support m1)) = (fid::lf,path++(idx::nil)) ->
+    sp_of_stack (Mem.stack (Mem.support m2)) = (lf,path).
+Proof.
+  intros. apply Mem.support_return_frame in H. unfold Mem.sup_return_frame in H.
+  destr_in H. destr_in H. unfold sp_of_stack in *. destr_in H0. inv H0.
+  destruct l. inv H2. assert (l<>nil).
+  destruct (Mem.stack (Mem.support m1)). destruct o.
+  simpl in Heqp1. destr_in Heqp1. inv Heqp1. apply sp_of_stack'_nonempty in Heqp.
+  destruct l2. congruence. inv H1. intro. destruct l2; inv H0.
+  inv Heqo.
+  apply exists_last in H0. destruct H0 as (l' & idx' & H0). subst.
+  exploit sp_of_stack_return'; eauto. intro. inv H. simpl. rewrite H0.
+  simpl in H2. destr_in H2. inv H2. auto.
+Qed.
+
+Lemma sp_of_stack_alloc' : forall st st' st'' path path0 path1 f lf pos id root,
+    next_stree st id = (st',path) ->
+    next_block_stree st' = (f,pos,path0,st'') ->
+    sp_of_stack' st = (lf++root::nil,path1) ->
+    exists idx,
+    sp_of_stack' st'' = (f::lf++root::nil,path0) /\ path0 = path1 ++ (idx::nil).
+Proof.
+  induction st. intros. destruct st. destruct o.
+  - simpl in H0. destr_in H0. inv H0. simpl in H1. repeat destr_in H1.
+    simpl in H2. destr_in H2.
+    apply sp_of_stack'_nonempty in Heqp1 as H0.
+    apply exists_last in H0. destruct H0 as (l' & a & H0). subst.
+    exploit H; eauto. simpl. auto.
+    intros (idx & A & B). exists idx. split. simpl. rewrite A.
+    inv H2. auto. inv H2. auto.
+  - simpl in H0. inv H0. simpl in H1. inv H1. simpl in H2. inv H2. simpl.
+    exists (length l0). auto.
+Qed.
+
+Lemma sp_of_stack_alloc : forall m1 m2 m3 id path lo hi b lf path',
+    Mem.alloc_frame m1 id = (m2,path) ->
+    Mem.alloc m2 lo hi = (m3,b) ->
+    sp_of_stack (Mem.stack (Mem.support m1)) = (lf,path') ->
+    exists idx, b = Stack (Some id) (path'++(idx::nil)) 1%positive /\
+    sp_of_stack (Mem.stack (Mem.support m3)) = ((Some id)::lf,path'++(idx::nil)).
+Proof.
+  intros.
+  exploit Mem.alloc_frame_alloc; eauto. intro.
+  apply Mem.path_alloc_frame in H as H'. unfold Mem.sup_npath in H'. unfold npath in H'.
+  apply Mem.support_alloc_frame in H. unfold Mem.sup_incr_frame in H.
+  destr_in H.
+  apply Mem.support_alloc in H0. unfold Mem.sup_incr in H0. destr_in H0.
+  rewrite H in Heqp0. simpl in Heqp0. destruct p0. destruct p0.
+  unfold sp_of_stack in *. destr_in H1.
+  apply sp_of_stack'_nonempty in Heqp2 as H3.
+  edestruct (exists_last H3) as (a & l' & H4). subst.
+  exploit sp_of_stack_alloc'; eauto. intros (idx & A& B).
+  exploit next_stree_next_block_stree; eauto. intros (X & Y & Z).
+  subst.
+  exists idx. split. inv H1. auto.
+  rewrite H0. simpl. rewrite A. simpl. inv H1. destr.
+Qed.
+
+Lemma sp_of_stack_external : forall m1 m2 ge ef vargs t vres,
+      external_call ef ge vargs m1 t vres m2 ->
+      sp_of_stack (Mem.stack (Mem.support m2)) = sp_of_stack (Mem.stack (Mem.support m1)).
+Admitted.
+
+(* maybe Vnullptr and Some (None,[]) is needed here*)
+
 Section RELSEM.
 
 (** Looking up instructions in a code sequence by position. *)
@@ -609,59 +781,6 @@ Definition exec_store (chunk: memory_chunk) (m: mem)
     the fact that the processor updates some or all of those flags,
     but we do not need to model this precisely.
 *)
-Definition aligned_fsz (sz:Z) := align (Z.max 0 sz) 8.
-
-Definition check_topframe (sz:Z)(astack:stackadt) : bool :=
-  match astack with
-    |nil => false
-    |top::tl => match top with
-                |fr::nil => if (zeq (aligned_fsz sz) (frame_size_a fr)) then true else false
-                |_ => false
-              end
-  end.
-
-Fixpoint sp_of_stack' (s:stree) : list fid * path :=
-  match s with
-   |Node fid bl l None => (fid::nil,nil)
-   |Node fid bl l (Some s') =>
-    let (lf',path') := sp_of_stack' s' in let idx := length bl in
-    ((fid::lf'),idx::path')
-  end.
-
-Definition sp_of_stack (s:stree) : list fid * path :=
-  let (lf,path) := (sp_of_stack' s) in (removelast lf,path).
-(* we have to ignore the root node*)
-Definition parent_sp_stree (st:stree) : val :=
-  let (lf,path) := sp_of_stack st in
-  match (lf,path) with
-    |(f1::((Some id)::tl), _::(_::_)) =>
-     Vptr (Stack (Some id) (removelast path) 1%positive) Ptrofs.zero
-    |_ => Vnullptr
-  end.
-
-Definition top_sp_stree (st:stree) : val :=
-  let (lf,path) := sp_of_stack st in
-  match (lf,path) with
-    | (((Some id)::tl), (_::_)) =>
-     Vptr (Stack (Some id) path 1%positive) Ptrofs.zero
-    |_ => Vnullptr
-  end.
-(*
-Definition parent_sp_stree (st:stree) : val :=
-  match parent_sp' st with
-    |Some(Some id,hd::tl) =>
-     Vptr (Stack (Some id) (hd::tl) 1%positive) Ptrofs.zero
-    |_ => Vnullptr
-  end.
-
-Definition top_sp_stree (st:stree) : val :=
-  match top_sp' st with
-    |((Some id),hd::tl) => Vptr (Stack (Some id) (hd::tl) 1%positive) Ptrofs.zero
-    |_ => Vnullptr
-  end.
-*)
-
-(* maybe Vnullptr and Some (None,[]) is needed here*)
 
 Definition exec_instr (f: function) (i: instruction) (rs: regset) (m: mem) : outcome :=
   match i with
